Improve memory proofmode tactics

imp_system/mem/MemTactics.v
@@ -194,6 +194,201 @@ Section mem.
   Qed.
 End mem.
 
+From iris.proofmode Require Import coq_tactics reduction spec_patterns.
+From iris.proofmode Require Export proofmode.
+From iris.bi Require Import derived_laws.
+Import bi.
+
+Section proofmode.
+  Context `{!crisG Γ Σ α β τ _S _I, !memGS}.
+
+  Local Definition pmem_state : Type := gmap key (option Any.t).
+  Local Definition pmem_post (R_s R_t : Type) : Type := pmem_state * R_s → pmem_state * R_t → iProp Σ.
+
+  Lemma tac_wsim_mem_load Δ i b ofs q v Δ2
+      fl_s fl_t Ist R_s R_t (RR : pmem_post R_s R_t) ps pt st_src st_tgt sp
+      (msk : emask) k_s k_t E1 E2 g :
+     fl_t !! fid MemHdr.load =
+      Some (Some (SB.sandbox_body
+        (msk, SModTr.trans_fnsem sp (fsp_some MemA.load, fbody_trivial)))) →
+    img_msk msk →
+    envs_lookup_delete true i Δ = Some (false, ((b, ofs) ↦{q} v)%I, Δ2) →
+    match envs_simple_replace i false (Esnoc Enil i (((b, ofs) ↦{q} v)%I)) Δ with
+    | Some Δ' =>
+      envs_entails Δ' (
+        wsim fl_s fl_t Ist (E1, E2) g R_s R_t RR ps true
+          (st_src, k_s)
+          (st_tgt, k_t v↑))
+    | None => False
+    end →
+    envs_entails Δ (
+      wsim fl_s fl_t Ist (E1, E2) g R_s R_t RR ps pt
+        (st_src, k_s)
+        (st_tgt, x <- trigger (Call MemHdr.load.1 [Vptr (b, ofs)]↑);; k_t x)).
+  Proof.
+    intros Hin Hmsk Hlook Hcont.
+    destruct (envs_simple_replace i false (Esnoc Enil i (((b, ofs) ↦{q} v)%I)) Δ)
+      as [Δ'|] eqn:Hrep; last done.
+    rewrite envs_entails_unseal in Hcont |- *.
+    apply envs_lookup_delete_Some in Hlook as [Hlook ->].
+    rewrite envs_lookup_sound' //=.
+    iIntros "[Hpt HΔ]".
+    iApply (wsim_mem_load with "Hpt"); eauto.
+    iIntros "Hpt".
+    iApply Hcont.
+    iApply (envs_simple_replace_sound' Δ Δ' i false
+      (Esnoc Enil i (((b, ofs) ↦{q} v)%I)) Hrep with "HΔ").
+    iFrame.
+  Unshelve. all: eauto.
+  Qed.
+
+  Lemma tac_wsim_mem_store Δ i b ofs v v' Δ2
+      fl_s fl_t Ist R_s R_t (RR : pmem_post R_s R_t) ps pt st_src st_tgt sp
+      (msk : emask) k_s k_t E1 E2 g :
+    fl_t !! fid MemHdr.store =
+      Some (Some (SB.sandbox_body
+        (msk, SModTr.trans_fnsem sp (fsp_some MemA.store, fbody_trivial)))) →
+    img_msk msk →
+    envs_lookup_delete true i Δ = Some (false, ((b, ofs) ↦ v')%I, Δ2) →
+    match envs_simple_replace i false (Esnoc Enil i (((b, ofs) ↦ v)%I)) Δ with
+    | Some Δ' =>
+      envs_entails Δ' (
+        wsim fl_s fl_t Ist (E1, E2) g R_s R_t RR ps true
+          (st_src, k_s)
+          (st_tgt, k_t (Vint 0)↑))
+    | None => False
+    end →
+    envs_entails Δ (
+      wsim fl_s fl_t Ist (E1, E2) g R_s R_t RR ps pt
+        (st_src, k_s)
+        (st_tgt, x <- trigger (Call MemHdr.store.1 [Vptr (b, ofs); v]↑);; k_t x)).
+  Proof.
+    intros Hin Hmsk Hlook Hcont.
+    destruct (envs_simple_replace i false (Esnoc Enil i (((b, ofs) ↦ v)%I)) Δ)
+      as [Δ'|] eqn:Hrep; last done.
+    rewrite envs_entails_unseal in Hcont |- *.
+    apply envs_lookup_delete_Some in Hlook as [Hlook ->].
+    rewrite envs_lookup_sound' //=.
+    iIntros "[Hpt HΔ]".
+    iApply (wsim_mem_store with "Hpt"); eauto.
+    iIntros "Hpt".
+    iApply Hcont.
+    iApply (envs_simple_replace_sound' Δ Δ' i false
+      (Esnoc Enil i (((b, ofs) ↦ v)%I)) Hrep with "HΔ").
+    iFrame.
+  Unshelve. all: eauto.
+  Qed.
+
+  Lemma tac_wsim_mem_free Δ i b ofs v' Δ2
+      fl_s fl_t Ist R_s R_t (RR : pmem_post R_s R_t) ps pt st_src st_tgt sp
+      (msk : emask) k_s k_t E1 E2 g :
+    fl_t !! fid MemHdr.free =
+      Some (Some (SB.sandbox_body
+        (msk, SModTr.trans_fnsem sp (fsp_some MemA.free, fbody_trivial)))) →
+    img_msk msk →
+    envs_lookup_delete true i Δ = Some (false, ((b, ofs) ↦ v')%I, Δ2) →
+    envs_entails Δ2 (
+      wsim fl_s fl_t Ist (E1, E2) g R_s R_t RR ps true
+        (st_src, k_s)
+        (st_tgt, k_t (Vint 0)↑)) →
+    envs_entails Δ (
+      wsim fl_s fl_t Ist (E1, E2) g R_s R_t RR ps pt
+        (st_src, k_s)
+        (st_tgt, x <- trigger (Call MemHdr.free.1 [Vptr (b, ofs)]↑);; k_t x)).
+  Proof.
+    rewrite envs_entails_unseal=> Hin Hmsk Hlook Hcont.
+    apply envs_lookup_delete_Some in Hlook as [Hlook ->].
+    rewrite envs_lookup_sound' //=.
+    iIntros "[Hpt HΔ]".
+    iApply (wsim_mem_free with "Hpt"); eauto.
+    iApply Hcont. iExact "HΔ".
+  Unshelve. all: eauto.
+  Qed.
+
+  Lemma tac_wsim_mem_cas Δ i b ofs v v_old v_new succ E Δ2
+      fl_s fl_t Ist R_s R_t (RR : pmem_post R_s R_t) ps pt st_src st_tgt sp
+      (msk : emask) k_s k_t E1 E2 g :
+    fl_t !! fid MemHdr.cas =
+      Some (Some (SB.sandbox_body
+        (msk, SModTr.trans_fnsem sp (fsp_some MemA.cas, fbody_trivial)))) →
+    img_msk msk →
+    envs_lookup_delete true i Δ = Some (false, ((b, ofs) ↦ v)%I, Δ2) →
+    MemA.compare_val v v_old = Vint succ →
+    envs_entails Δ2 (
+      E ∗
+      (E ==∗ ∃ q0 q1 v0 v1, MemA.val_r v q0 v0 ∗ MemA.val_r v_old q1 v1 ∗
+            (MemA.val_r v q0 v0 ∗ MemA.val_r v_old q1 v1 ==∗ E)) ∗
+      (((b, ofs) ↦ if (bool_decide (succ = 1)) then v_new else v) -∗
+       E -∗
+        wsim fl_s fl_t Ist (E1, E2) g R_s R_t RR ps true
+          (st_src, k_s)
+          (st_tgt, k_t v↑))) →
+    envs_entails Δ (
+      wsim fl_s fl_t Ist (E1, E2) g R_s R_t RR ps pt
+        (st_src, k_s)
+        (st_tgt, x <- trigger (Call MemHdr.cas.1 [Vptr (b, ofs); v_old; v_new]↑);; k_t x)).
+  Proof.
+    rewrite envs_entails_unseal=> Hin Hmsk Hlook Hcmp Hcont.
+    apply envs_lookup_delete_Some in Hlook as [Hlook ->].
+    rewrite envs_lookup_sound' //=.
+    iIntros "[Hpt HΔ]".
+    iPoseProof (Hcont with "HΔ") as "[E [HE K]]".
+    iApply (wsim_mem_cas with "Hpt E HE K"); eauto.
+  Unshelve. all: eauto.
+  Qed.
+
+  Lemma tac_wsim_mem_cmp Δ v1 v2 succ E
+      fl_s fl_t Ist R_s R_t (RR : pmem_post R_s R_t) ps pt st_src st_tgt sp
+      (msk : emask) k_s k_t E1 E2 g :
+    fl_t !! (fid MemHdr.cmp) =
+      Some (Some (SB.sandbox_body
+        (msk, SModTr.trans_fnsem sp (fsp_some (MemA.cmp), fbody_trivial)))) →
+    img_msk msk →
+    MemA.compare_val v1 v2 = Vint succ →
+    envs_entails Δ (
+      E ∗
+      (E ==∗ ∃ q0 q1 v1' v2', MemA.val_r v1 q0 v1' ∗ MemA.val_r v2 q1 v2' ∗
+            (MemA.val_r v1 q0 v1' ∗ MemA.val_r v2 q1 v2' ==∗ E)) ∗
+      (E -∗
+        wsim fl_s fl_t Ist (E1, E2) g R_s R_t RR ps true
+          (st_src, k_s)
+          (st_tgt, k_t (Vint succ)↑))) →
+    envs_entails Δ (
+      wsim fl_s fl_t Ist (E1, E2) g R_s R_t RR ps pt
+        (st_src, k_s)
+        (st_tgt, x <- trigger (Call MemHdr.cmp.1 [v1; v2]↑);; k_t x)).
+  Proof.
+    rewrite envs_entails_unseal=> Hin Hmsk Hcmp Hcont.
+    rewrite Hcont.
+    iIntros "[E [HE K]]".
+    iApply (wsim_mem_cmp with "E HE K"); eauto.
+  Unshelve. all: eauto.
+  Qed.
+
+  Lemma tac_wsim_mem_cmp_int Δ n1 n2
+      fl_s fl_t Ist R_s R_t (RR : pmem_post R_s R_t) ps pt st_src st_tgt sp
+      (msk : emask) k_s k_t E1 E2 g :
+    fl_t !! (fid MemHdr.cmp) =
+      Some (Some (SB.sandbox_body
+        (msk, SModTr.trans_fnsem sp (fsp_some (MemA.cmp), fbody_trivial)))) →
+    img_msk msk →
+    envs_entails Δ (
+      wsim fl_s fl_t Ist (E1, E2) g R_s R_t RR ps true
+        (st_src, k_s)
+        (st_tgt, k_t (Vint (if decide (n1 = n2) then 1 else 0)%Z)↑)) →
+    envs_entails Δ (
+      wsim fl_s fl_t Ist (E1, E2) g R_s R_t RR ps pt
+        (st_src, k_s)
+        (st_tgt, x <- trigger (Call MemHdr.cmp.1 [Vint n1; Vint n2]↑);; k_t x)).
+  Proof.
+    rewrite envs_entails_unseal=> Hin Hmsk Hcont.
+    rewrite Hcont.
+    iIntros "K".
+    iApply (wsim_mem_cmp_int with "K"); eauto.
+  Unshelve. all: eauto.
+  Qed.
+End proofmode.
+
 Tactic Notation "mLoadT" uconstr(H) :=
   iApply (wsim_mem_load with H); [try by simpl_map|ss|]; last (iIntros H; cStepsT).
 Tactic Notation "mStoreT" uconstr(H) :=
@@ -202,3 +397,71 @@ Tactic Notation "mAllocT" "as" "(" simple_intropattern(x) ")" uconstr(H) :=
   iApply wsim_mem_alloc; [try by simpl_map|ss|ss|iIntros (x) H; cStepsT].
 Tactic Notation "mFreeT" uconstr(H) :=
   iApply (wsim_mem_free with H); [try by simpl_map|ss|cStepsT].
+
+Tactic Notation "mLoad" :=
+  eapply tac_wsim_mem_load;
+    [try by simpl_map
+    |ss
+    |iAssumptionCore || fail "mLoad: no matching ↦"
+    |pm_reduce; cStepsT].
+
+Tactic Notation "mStore" :=
+  eapply tac_wsim_mem_store;
+    [try by simpl_map
+    |ss
+    |iAssumptionCore || fail "mStore: no matching ↦"
+    |pm_reduce; cStepsT].
+
+Tactic Notation "mFree" :=
+  eapply tac_wsim_mem_free;
+    [try by simpl_map
+    |ss
+    |iAssumptionCore || fail "mFree: no matching ↦"
+    |pm_reduce; cStepsT].
+
+Tactic Notation "mCas" :=
+  eapply tac_wsim_mem_cas;
+    [try solve [simpl_map | prove_inline_cond | prove_sb_cond | ss]
+    |ss
+    |iAssumptionCore || fail "mCas: no matching ↦"
+    |try solve [eauto | rewrite /MemA.compare_val; des_ifs; eauto]
+    |pm_reduce].
+
+Tactic Notation "mCas" constr(succ) :=
+  eapply (tac_wsim_mem_cas _ _ _ _ _ _ _ succ);
+    [try solve [simpl_map | prove_inline_cond | prove_sb_cond | ss]
+    |ss
+    |iAssumptionCore || fail "mCas: no matching ↦"
+    |try solve [eauto | rewrite /MemA.compare_val; des_ifs; eauto]
+    |pm_reduce].
+
+Tactic Notation "mCmp" :=
+  eapply tac_wsim_mem_cmp;
+    [try solve [simpl_map | prove_inline_cond | prove_sb_cond | ss]
+    |ss
+    |try solve [eauto | rewrite /MemA.compare_val; des_ifs; eauto]
+    |pm_reduce].
+
+Tactic Notation "mCmp" constr(succ) :=
+  eapply (tac_wsim_mem_cmp _ _ _ succ);
+    [try solve [simpl_map | prove_inline_cond | prove_sb_cond | ss]
+    |ss
+    |try solve [eauto | rewrite /MemA.compare_val; des_ifs; eauto]
+    |pm_reduce].
+
+Tactic Notation "mCmpInt" :=
+  eapply tac_wsim_mem_cmp_int;
+    [try by simpl_map
+    |ss
+    |cStepsT].
+
+Tactic Notation "mStep" :=
+  lazymatch goal with
+  | |- environments.envs_entails _
+      (wsim _ _ _ _ _ _ _ _ _ _
+        (_, _)
+        (_, _)) =>
+    first [mLoad | mStore | mFree | mCas | mCmpInt | mCmp]
+  end.
+
+Tactic Notation "mSteps" := repeat (mStep; try cStepsT).
